Janus1.v
@@ -37,7 +37,8 @@ Section Janus1.
     | Exp_Or    : Exp -> Exp -> Exp
     | Exp_Lt    : Exp -> Exp -> Exp.
 
-    Fixpoint denote_Exp (m : W32Mem.memory) (e : Exp) {struct e} : option w32 :=
+    Fixpoint denote_Exp (m : W32Mem.memory) (e : Exp) {struct e}
+        : option w32 :=
       match e with
         | Exp_Const z => Some z
         | Exp_Var x => m x
@@ -69,13 +70,17 @@ Section Janus1.
         | Exp_Eq e1 e2 =>
           match (denote_Exp m e1, denote_Exp m e2) with
             | (Some n1, Some n2) =>
-                Some (if Word32.cmpu Ceq n1 n2 then Word32.one else Word32.zero)
+                Some (if Word32.cmpu Ceq n1 n2
+                      then Word32.one
+                      else Word32.zero)
             | _ => None
           end
         | Exp_Neq e1 e2 =>
           match (denote_Exp m e1, denote_Exp m e2) with
             | (Some n1, Some n2) =>
-                Some (if Word32.cmpu Cne n1 n2 then Word32.one else Word32.zero)
+                Some (if Word32.cmpu Cne n1 n2
+                      then Word32.one
+                      else Word32.zero)
             | _ => None
           end
         | Exp_And e1 e2 =>
@@ -101,36 +106,55 @@ Section Janus1.
         | Exp_Lt e1 e2 =>
           match (denote_Exp m e1, denote_Exp m e2) with
             | (Some n, Some n') =>
-              Some (if Word32.cmpu Clt n n' then Word32.one else Word32.zero)
+              Some (if Word32.cmpu Clt n n'
+                    then Word32.one
+                    else Word32.zero)
             | _ => None
           end
       end.
 
     Definition exp_equiv (e1: Exp) (e2: Exp) :=
       forall (v: Value) (m: W32Mem.memory),
-        denote_Exp m e1 = Some v <-> denote_Exp m e2 = Some v.
+        denote_Exp m e1 = Some v
+        <->
+        denote_Exp m e2 = Some v.
 
     Lemma exp_equiv_refl: forall e, exp_equiv e e.
-    Proof. unfold exp_equiv. grind. Qed.
-
-    Lemma exp_equiv_sym: forall e1 e2, exp_equiv e1 e2 <-> exp_equiv e2 e1.
     Proof.
-      unfold exp_equiv. intros. split. intros. symmetry. eapply H.
-                                       intros. symmetry. eapply H.
+      unfold exp_equiv. grind.
+    Qed.
+
+    Lemma exp_equiv_sym: forall e1 e2,
+      exp_equiv e1 e2 <-> exp_equiv e2 e1.
+    Proof.
+      unfold exp_equiv.
+      intros. split. intros.
+      symmetry.
+      eapply H.
+      intros.
+      symmetry.
+      eapply H.
     Qed.
 
     Lemma exp_equiv_tr: forall e1 e2 e3,
       exp_equiv e1 e2 -> exp_equiv e2 e3 -> exp_equiv e1 e3.
     Proof.
       unfold exp_equiv. intros.
-      split. intro. assert (denote_Exp m e2 = Some v). eapply H. eauto.
-                    eapply H0. eauto.
-             intro. assert (denote_Exp m e2 = Some v). eapply H0. eauto.
-                    eapply H. eauto.
+      split.
+      intro.
+      assert (denote_Exp m e2 = Some v).
+        eapply H. eauto.
+        eapply H0. eauto.
+      intro.
+      assert (denote_Exp m e2 = Some v).
+        eapply H0. eauto.
+        eapply H. eauto.
     Qed.
 
     Theorem exp_determ : forall m e v1 v2,
-      denote_Exp m e = v1 -> denote_Exp m e = v2 -> v1 = v2.
+      denote_Exp m e = v1
+      -> denote_Exp m e = v2
+      -> v1 = v2.
     Proof.
       grind.
     Qed.
@@ -154,47 +178,55 @@ Section Janus1.
 
     Inductive Stm_eval : defs -> mem -> Stm -> mem -> Prop :=
     | se_skip: forall d m, Stm_eval d m S_Skip m
-    | se_assvar_incr: forall (d : defs) (m m': mem) (v: Var) (z z' r: w32) (e: Exp),
+    | se_assvar_incr: forall (d : defs) (m m': mem)
+        (v: Var) (z z' r: w32) (e: Exp),
       denote_Exp (W32Mem.hide m v) e = Some z ->
       m v = Some z' ->
       r = (Word32.add z z') ->
       m' = W32Mem.write m v r ->
       Stm_eval d m (S_Incr v e) m'
-    | se_assvar_decr: forall (d : defs) (m m': mem) (v: Var) (z z' r: w32) (e: Exp),
+    | se_assvar_decr: forall (d : defs) (m m': mem)
+        (v: Var) (z z' r: w32) (e: Exp),
       denote_Exp (W32Mem.hide m v) e = Some z ->
       m v = Some z' ->
       r = (Word32.sub z' z) ->
       m' = W32Mem.write m v r ->
       Stm_eval d m (S_Decr v e) m'
-    | se_assvar_xor: forall (d : defs) (m m': mem) (v: Var) (n n' n'': w32) (e: Exp),
+    | se_assvar_xor: forall (d : defs) (m m': mem)
+        (v: Var) (n n' n'': w32) (e: Exp),
       denote_Exp (W32Mem.hide m v) e = Some n ->
       m v = Some n' ->
       Word32.xor n n' = n'' ->
       m' = W32Mem.write m v n'' ->
       Stm_eval d m (S_Xor v e) m'
-    | se_semi: forall (d : defs) (m m' m'': mem) (s1 s2: Stm),
+    | se_semi: forall (d : defs) (m m' m'': mem)
+        (s1 s2: Stm),
       Stm_eval d m s1 m' ->
       Stm_eval d m' s2 m'' ->
       Stm_eval d m (S_Semi s1 s2) m''
-    | se_if_t: forall (d : defs) (m m': mem) (e1 e2: Exp) (s1 s2: Stm) (k k': w32),
+    | se_if_t: forall (d : defs) (m m': mem)
+        (e1 e2: Exp) (s1 s2: Stm) (k k': w32),
       denote_Exp m e1 = Some k ->
       Word32.is_true(k) ->
       Stm_eval d m s1 m' ->
       denote_Exp m' e2 = Some k' ->
       Word32.is_true(k') ->
       Stm_eval d m (S_If e1 s1 s2 e2) m'
-    | se_if_f: forall (d : defs) (m m': mem) (e1 e2: Exp) (s1 s2: Stm) (k k': w32),
+    | se_if_f: forall (d : defs) (m m': mem)
+        (e1 e2: Exp) (s1 s2: Stm) (k k': w32),
       denote_Exp m e1 = Some k ->
       Word32.is_false(k) ->
       Stm_eval d m s2 m' ->
       denote_Exp m' e2 = Some k' ->
       Word32.is_false(k') ->
       Stm_eval d m (S_If e1 s1 s2 e2) m'
-    | se_call: forall (d : defs) (v : Z) (m m' : mem) (s : Stm),
+    | se_call: forall (d : defs) (v : Z) (m m' : mem)
+        (s : Stm),
       d v = s ->
       Stm_eval d m s m' ->
       Stm_eval d m (S_Call v) m'
-    | se_uncall: forall (d : defs) (v : Z) (m m' : mem) (s : Stm),
+    | se_uncall: forall (d : defs) (v : Z) (m m' : mem)
+        (s : Stm),
       d v = s ->
       Stm_eval d m' s m ->
       Stm_eval d m (S_Uncall v) m'.
@@ -224,28 +256,37 @@ Section Janus1.
     Qed.
 
     Lemma semi_assoc: forall s1 s2 s3,
-      stm_equiv (S_Semi (S_Semi s1 s2) s3) (S_Semi s1 (S_Semi s2 s3)).
+      stm_equiv (S_Semi (S_Semi s1 s2) s3)
+                (S_Semi s1 (S_Semi s2 s3)).
     Proof.
       intros. unfold stm_equiv. grind.
       inversion H. inversion H4. subst.
-        assert (Stm_eval d m'1 (S_Semi s2 s3) m'). constructor 5 with (m' := m'0);
-          assumption. constructor 5 with (m' := m'1); assumption.
-      inversion H. subst. inversion H6. subst.
-        assert (Stm_eval d m (S_Semi s1 s2) m'1). constructor 5 with (m' := m'0);
+        assert (Stm_eval d m'1 (S_Semi s2 s3) m').
+        constructor 5 with (m' := m'0);
           assumption.
+        constructor 5 with (m' := m'1);
+          assumption.
+      inversion H. subst. inversion H6. subst.
+        assert (Stm_eval d m (S_Semi s1 s2) m'1).
+          constructor 5 with (m' := m'0);
+            assumption.
         constructor 5 with (m' := m'1); assumption.
     Qed.
 
     Definition fwd_det G m s m' :=
-      Stm_eval G m s m' -> forall m'', Stm_eval G m s m'' -> m' = m''.
+      Stm_eval G m s m' ->
+        forall m'', Stm_eval G m s m'' -> m' = m''.
 
     Definition bwd_det G m s m' :=
-      Stm_eval G m s m' -> forall m'', Stm_eval G m'' s m' -> m = m''.
+      Stm_eval G m s m' ->
+        forall m'', Stm_eval G m'' s m' -> m = m''.
 
     Lemma b_forward_det: forall G m s m',
       (forall G m s m', bwd_det G m s m') -> fwd_det G m s m'.
     Proof.
-      unfold fwd_det. intros until m'. intro. induction 1; intros.
+      unfold fwd_det. intros until m'.
+      intro. induction 1; intros.
+
       inversion H0. intuition.
 
       inversion H4. subst.
@@ -260,11 +301,20 @@ Section Janus1.
       assert (n = n0). grind.
       assert (n' = n'0). grind. grind.
 
-      inversion H0. subst. apply IHStm_eval2. assert (m' = m'0). eapply IHStm_eval1. eauto.
+      inversion H0. subst. apply IHStm_eval2.
+      assert (m' = m'0).
+        eapply IHStm_eval1. eauto.
       subst. trivial.
 
-      inversion H5. subst. apply (IHStm_eval m''). trivial. congruence.
-      inversion H5. subst. congruence. subst. apply (IHStm_eval m''). trivial.
+      inversion H5. subst.
+      apply (IHStm_eval m'').
+      trivial.
+      congruence.
+      inversion H5.
+      subst.
+      congruence.
+      subst.
+      apply (IHStm_eval m''). trivial.
 
       inversion H2. subst. apply IHStm_eval. trivial.
       inversion H2. subst. eapply H. eauto. trivial.
@@ -277,37 +327,68 @@ Section Janus1.
       inversion H0. trivial.
 
       inversion H4. subst.
-      assert (W32Mem.hide m v = W32Mem.hide m'' v). eapply W32Mem.write_hide. eauto.
-      assert (Word32.add z z' = Word32.add z0 z'0). assert (W32Mem.write m v (Word32.add z z') v = W32Mem.write m'' v (Word32.add z0 z'0) v).
-      apply equal_f. trivial. apply (W32Mem.write_eq_2 m m'' v). trivial.
-      assert (z = z0). assert (Some z = Some z0). grind. grind.
+      assert (W32Mem.hide m v = W32Mem.hide m'' v).
+        eapply W32Mem.write_hide. eauto.
+      assert (Word32.add z z' = Word32.add z0 z'0).
+      assert (W32Mem.write m v (Word32.add z z') v =
+              W32Mem.write m'' v (Word32.add z0 z'0) v).
+      apply equal_f. trivial.
+      apply (W32Mem.write_eq_2 m m'' v). trivial.
+      assert (z = z0).
+      assert (Some z = Some z0).
+        grind.
+        grind.
       subst.
-      assert (z' = z'0). eapply Word32.add_eq_r. eauto.
-      subst. apply (W32Mem.hide_eq m m'' v z'0). trivial. trivial. trivial.
+      assert (z' = z'0).
+        eapply Word32.add_eq_r. eauto.
+      subst.
+      apply (W32Mem.hide_eq m m'' v z'0).
+      trivial.
+      trivial.
+      trivial.
 
       inversion H4. subst.
-      assert (W32Mem.hide m v = W32Mem.hide m'' v). eapply W32Mem.write_hide. eauto.
+      assert (W32Mem.hide m v = W32Mem.hide m'' v).
+        eapply W32Mem.write_hide. eauto.
       assert (Word32.sub z' z = Word32.sub z'0 z0).
-      assert (W32Mem.write m v (Word32.sub z' z) v = W32Mem.write m'' v (Word32.sub z'0 z0) v).
-      apply equal_f. trivial. apply (W32Mem.write_eq_2 m m'' v). trivial.
-      assert (z = z0). assert (Some z = Some z0); grind.
-      assert (z' = z'0). subst. eapply Word32.sub_eq_l. eauto.
-      subst. apply (W32Mem.hide_eq m m'' v z'0). trivial. trivial. trivial.
+      assert (W32Mem.write m v (Word32.sub z' z) v =
+              W32Mem.write m'' v (Word32.sub z'0 z0) v).
+      apply equal_f. trivial.
+      apply (W32Mem.write_eq_2 m m'' v). trivial.
+      assert (z = z0).
+      assert (Some z = Some z0); grind.
+      assert (z' = z'0).
+        subst. eapply Word32.sub_eq_l. eauto.
+      subst. apply (W32Mem.hide_eq m m'' v z'0).
+      trivial.
+      trivial.
+      trivial.
 
       inversion H4. subst.
-      assert (W32Mem.hide m v = W32Mem.hide m'' v). eapply W32Mem.write_hide. eauto.
-      assert (Word32.xor n n' = Word32.xor n0 n'0). assert (W32Mem.write m v (Word32.xor n n') v = W32Mem.write m'' v (Word32.xor n0 n'0) v).
-      apply equal_f. trivial. eapply W32Mem.write_eq_2. eauto.
-      assert (n = n0). assert (Some n = Some n0). rewrite H2 in H0. congruence. grind.
+      assert (W32Mem.hide m v = W32Mem.hide m'' v).
+        eapply W32Mem.write_hide. eauto.
+      assert (Word32.xor n n' = Word32.xor n0 n'0).
+        assert (W32Mem.write m v (Word32.xor n n') v =
+                W32Mem.write m'' v (Word32.xor n0 n'0) v).
+      apply equal_f. trivial.
+        eapply W32Mem.write_eq_2. eauto.
+      assert (n = n0).
+      assert (Some n = Some n0).
+      rewrite H2 in H0. congruence. grind.
       subst.
-      assert (n'0 = n'). eapply Word32.xor_mine. eauto.
-      subst. eapply (W32Mem.hide_eq m m'' v); eauto.
+      assert (n'0 = n').
+        eapply Word32.xor_mine. eauto.
+      subst.
+        eapply (W32Mem.hide_eq m m'' v); eauto.
 
-      inversion H0. subst. assert (m' = m'0). apply IHStm_eval2. trivial.
+      inversion H0. subst.
+      assert (m' = m'0). apply IHStm_eval2. trivial.
       subst. apply IHStm_eval1. trivial.
 
-      inversion H5. subst. apply IHStm_eval. trivial. congruence.
-      inversion H5. subst. congruence. apply IHStm_eval. trivial.
+      inversion H5.
+        subst. apply IHStm_eval. trivial. congruence.
+      inversion H5.
+        subst. congruence. apply IHStm_eval. trivial.
 
       inversion H2. subst. apply IHStm_eval. trivial.
 
@@ -353,33 +434,72 @@ Section Janus1.
       apply (W32Mem.hide_eq m (W32Mem.write m' v (Word32.sub r z)) v z').
         assumption.
         assert (Word32.sub r z = z').
-          rewrite H1. rewrite Word32.add_commut. rewrite Word32.sub_add_opp.
-          rewrite Word32.add_assoc. rewrite Word32.add_neg_zero. rewrite Word32.add_zero. trivial.
-        rewrite H3. apply W32Mem.write_eq.
-        rewrite W32Mem.hide_write. rewrite H2. rewrite W32Mem.hide_write.
+          rewrite H1.
+          rewrite Word32.add_commut.
+          rewrite Word32.sub_add_opp.
+          rewrite Word32.add_assoc.
+          rewrite Word32.add_neg_zero.
+          rewrite Word32.add_zero.
+          trivial.
+        rewrite H3.
+        apply W32Mem.write_eq.
+        rewrite W32Mem.hide_write.
+        rewrite H2.
+        rewrite W32Mem.hide_write.
         trivial.
       simpl.
       apply (se_assvar_incr d m' m v z r (Word32.add r z)).
-        rewrite H2. rewrite W32Mem.hide_write. assumption.
-        rewrite H2. apply W32Mem.write_eq. rewrite Word32.add_commut. trivial.
+        rewrite H2.
+        rewrite W32Mem.hide_write.
+        assumption.
+        rewrite H2.
+        apply W32Mem.write_eq.
+        rewrite Word32.add_commut.
+        trivial.
       apply (W32Mem.hide_eq m (W32Mem.write m' v (Word32.add r z)) v z').
-        trivial. rewrite W32Mem.write_eq. assert (Word32.add r z = z').
-          rewrite H1. rewrite Word32.sub_add_opp. rewrite Word32.add_assoc.
-          assert (Word32.add (Word32.neg z) z = Word32.add z (Word32.neg z)).
-            apply Word32.add_commut. rewrite H3. clear H3. rewrite Word32.add_neg_zero.
-            rewrite Word32.add_zero. trivial.
-        rewrite H3. trivial.
-        rewrite W32Mem.hide_write. rewrite H2. rewrite W32Mem.hide_write. trivial.
+        trivial.
+        rewrite W32Mem.write_eq.
+        assert (Word32.add r z = z').
+          rewrite H1.
+          rewrite Word32.sub_add_opp.
+          rewrite Word32.add_assoc.
+          assert (Word32.add (Word32.neg z) z =
+                  Word32.add z (Word32.neg z)).
+            apply Word32.add_commut.
+            rewrite H3.
+            clear H3.
+            rewrite Word32.add_neg_zero.
+            rewrite Word32.add_zero.
+            trivial.
+            rewrite H3.
+            trivial.
+        rewrite W32Mem.hide_write.
+        rewrite H2.
+        rewrite W32Mem.hide_write.
+        trivial.
       simpl. apply (se_assvar_xor d m' m v n n'' n').
-        rewrite H2. rewrite W32Mem.hide_write. assumption.
-        rewrite H2. apply W32Mem.write_eq.
+        rewrite H2.
+        rewrite W32Mem.hide_write.
+        assumption.
+        rewrite H2.
+        apply W32Mem.write_eq.
         assert (n' = Word32.xor n n'').
-        rewrite <- H1. rewrite <- Word32.xor_assoc. rewrite Word32.xor_x_x_zero.
-        rewrite Word32.xor_commut. rewrite Word32.xor_zero. trivial.
-        symmetry. trivial.
-      apply (W32Mem.hide_eq m (W32Mem.write m' v n') v n'). trivial.
-        rewrite W32Mem.write_eq. trivial. rewrite W32Mem.hide_write. rewrite H2.
-        rewrite W32Mem.hide_write. trivial.
+        rewrite <- H1.
+        rewrite <- Word32.xor_assoc.
+        rewrite Word32.xor_x_x_zero.
+        rewrite Word32.xor_commut.
+        rewrite Word32.xor_zero.
+        trivial.
+        symmetry.
+        trivial.
+      apply (W32Mem.hide_eq m (W32Mem.write m' v n') v n').
+        trivial.
+        rewrite W32Mem.write_eq.
+        trivial.
+        rewrite W32Mem.hide_write.
+        rewrite H2.
+        rewrite W32Mem.hide_write.
+        trivial.
 
       simpl. eapply se_semi. eauto. trivial.
       simpl. eapply se_if_t; eauto.
@@ -391,44 +511,90 @@ Section Janus1.
       intros.
       simpl in H. inversion H.
       apply (se_assvar_incr G m0 m'0 v z r (Word32.add r z)).
-        rewrite H8. rewrite W32Mem.hide_write. assumption.
-        rewrite H8. apply W32Mem.write_eq. rewrite Word32.add_commut. trivial.
+        rewrite H8.
+        rewrite W32Mem.hide_write.
+        assumption.
+        rewrite H8.
+        apply W32Mem.write_eq.
+        rewrite Word32.add_commut.
+        trivial.
       apply (W32Mem.hide_eq  m'0 (W32Mem.write m0 v (Word32.add r z)) v z').
         trivial.
-        rewrite W32Mem.write_eq. rewrite H6. assert (z' = Word32.add (Word32.sub z' z) z).
-          rewrite Word32.sub_add_opp. rewrite Word32.add_commut. rewrite Word32.add_permut.
-          rewrite Word32.add_neg_zero. rewrite Word32.add_zero. trivial.
-          rewrite <- H9. trivial.
-          rewrite W32Mem.hide_write. rewrite H8. rewrite W32Mem.hide_write.
+        rewrite W32Mem.write_eq.
+        rewrite H6.
+        assert (z' = Word32.add (Word32.sub z' z) z).
+          rewrite Word32.sub_add_opp.
+          rewrite Word32.add_commut.
+          rewrite Word32.add_permut.
+          rewrite Word32.add_neg_zero.
+          rewrite Word32.add_zero.
+          trivial.
+          rewrite <- H9.
+          trivial.
+          rewrite W32Mem.hide_write.
+          rewrite H8.
+          rewrite W32Mem.hide_write.
           trivial.
       intros.
       simpl in H. inversion H.
       apply (se_assvar_decr G m0 m'0 v z r (Word32.sub r z)).
-        rewrite H8. rewrite W32Mem.hide_write. trivial.
-        rewrite H8. apply W32Mem.write_eq. trivial.
-        apply (W32Mem.hide_eq m'0 (W32Mem.write m0 v (Word32.sub r z)) v z').
+        rewrite H8.
+        rewrite W32Mem.hide_write.
         trivial.
-        assert (Word32.sub r z = z'). rewrite H6. rewrite Word32.sub_add_opp.
-        rewrite Word32.add_commut. rewrite <- Word32.add_assoc.
-        assert (Word32.add (Word32.neg z) z = Word32.add z (Word32.neg z)).
-        apply Word32.add_commut. rewrite H9. clear H9. rewrite Word32.add_neg_zero.
-        rewrite Word32.add_commut. rewrite Word32.add_zero. trivial.
-        rewrite H9. apply W32Mem.write_eq.
-        rewrite W32Mem.hide_write. rewrite H8. rewrite W32Mem.hide_write.
+        rewrite H8.
+        apply W32Mem.write_eq.
+        trivial.
+        apply (W32Mem.hide_eq m'0 
+           (W32Mem.write m0 v (Word32.sub r z)) v z').
+        trivial.
+        assert (Word32.sub r z = z').
+        rewrite H6.
+        rewrite Word32.sub_add_opp.
+        rewrite Word32.add_commut.
+        rewrite <- Word32.add_assoc.
+        assert (Word32.add (Word32.neg z) z =
+                Word32.add z (Word32.neg z)).
+        apply Word32.add_commut.
+        rewrite H9.
+        clear H9.
+        rewrite Word32.add_neg_zero.
+        rewrite Word32.add_commut.
+        rewrite Word32.add_zero.
+        trivial.
+        rewrite H9.
+        apply W32Mem.write_eq.
+        rewrite W32Mem.hide_write.
+        rewrite H8.
+        rewrite W32Mem.hide_write.
         trivial.
       intros.
         simpl in H. inversion H.
       apply (se_assvar_xor G m0 m'0 v n n'' n').
-        rewrite H8. rewrite W32Mem.hide_write. assumption.
-        rewrite H8. apply W32Mem.write_eq.
+        rewrite H8.
+        rewrite W32Mem.hide_write. assumption.
+        rewrite H8.
+        apply W32Mem.write_eq.
         assert (n' = Word32.xor n n'').
-        rewrite <- H6. rewrite <- Word32.xor_assoc. rewrite Word32.xor_x_x_zero.
-        rewrite Word32.xor_commut. rewrite Word32.xor_zero. trivial.
-        symmetry. trivial. 
-        apply (W32Mem.hide_eq m'0 (W32Mem.write m0 v n') v n'). trivial. apply W32Mem.write_eq.
-        rewrite W32Mem.hide_write. rewrite H8. rewrite W32Mem.hide_write. trivial.
+        rewrite <- H6.
+        rewrite <- Word32.xor_assoc.
+        rewrite Word32.xor_x_x_zero.
+        rewrite Word32.xor_commut.
+        rewrite Word32.xor_zero.
+        trivial.
+        symmetry.
+        trivial.
+        apply (W32Mem.hide_eq m'0
+          (W32Mem.write m0 v n') v n').
+        trivial.
+        apply W32Mem.write_eq.
+        rewrite W32Mem.hide_write.
+        rewrite H8.
+        rewrite W32Mem.hide_write.
+        trivial.
       intros.
-      inversion H. apply (se_semi G m0 m'1 m'0). apply IHs1. trivial.
+      inversion H.
+      apply (se_semi G m0 m'1 m'0).
+      apply IHs1. trivial.
         apply IHs2. trivial.
       intros.
         inversion H. eapply se_if_t; eauto. eapply se_if_f; eauto.
